extraction/extraction.v
@@ -90,6 +90,7 @@ Extract Constant Allocation.regalloc => "Regalloc.regalloc".
 Extract Constant Linearize.enumerate_aux => "Linearizeaux.enumerate_aux".
 
 (* SimplExpr *)
+Extract Constant MoSel.gensym.first_unused_ident => "Camlcoq.first_unused_ident".
 Extraction Inline MoSel.gensym.run.
 
 (* Compopts *)
